@prefix : <http://www.seqweb.org/> .
@prefix seq: <http://www.seqweb.org/> .
@prefix oeis: <http://www.oeis.org/> .
@prefix owl: <http://www.w3.org/2002/07/owl#> .
@prefix rdfs: <http://www.w3.org/2000/01/rdf-schema#> .
@prefix rdf: <http://www.w3.org/1999/02/22-rdf-syntax-ns#> .
@prefix cnt: <http://www.w3.org/2011/content#> .

:Text a rdfs:Class ;
    rdfs:subClassOf cnt:ContentAsText ,
        [ a owl:Restriction ;
          owl:onProperty cnt:characterEncoding ;
          owl:hasValue "utf-8"
        ] ;
    rdfs:label "Text block with assumed UTF-8 encoding"@en ;
    rdfs:comment "DRYer synonym for cnt:ContentAsText where encoding is assumed UTF-8."@en .


:Sequence a owl:Class ;
    rdfs:label "Sequence"@en ;
    rdfs:comment "An OEIS and mathematical integer sequence modeled in the SeqWeb knowledge graph."@en . 

:hasTextList a owl:ObjectProperty ;
    rdfs:domain :Sequence ;
    rdfs:range rdf:List ;
    # owl:inverseOf :isTextListOf ;
    rdfs:comment "Links a Sequence to an ordered list of :Text blocks."@en .

# :isTextListOf a owl:ObjectProperty ;
#     rdfs:domain rdf:List ;
#     rdfs:range :Sequence ;
#     owl:inverseOf :hasTextList ;
#     rdfs:comment "Links an ordered list of :Text blocks to the Sequence they belong to."@en .
